Soit \(\beta = \{u_{1}, \ldots, u_{s^{2}}\}\) une base orthonormée de \(\mathbb{R}^{s^{2}}\).\\
On notera ici \(u\) un vecteur de \(\beta\) et \(u^{\top}\) sa transposée. \\

Soit \(x = V(k) - m(v) \in \mathbb{R}^{s^{2}}\).

On a :
\[
x = \sum_{i=1}^{s^{2}} \beta_{i} u_{i}
\]

De plus :
\[
\langle x \mid u_{j} \rangle = \left\langle \sum_{i=1}^{s^{2}} \beta_{i} u_{i} \big{|} u_{j} \right\rangle = \sum_{i=1}^{s^{2}} \beta_{i} \langle u_{i} \mid u_{j} \rangle = \beta_{j} \langle u_{j} \mid u_{j} \rangle = \beta_{j}
\]

Donc :
\[
\beta_{i} = \langle x \mid u_{i} \rangle
\]

Ainsi :
\[
V(k) - m(v) = \sum_{i=1}^{s^{2}} \langle V(k) - m(v) \mid u_{i} \rangle \, u_{i} = \sum_{i=1}^{s^{2}} u_{i}^{\top} \left( V(k) - m(v) \right) u_{i}
\]

Finalement :
\[
V(k) = m(v) + \sum_{i=1}^{s^{2}} u_{i}^{\top} \left( V(k) - m(v) \right) u_{i}
\]